Some steps proof WF properties interface + invariants

examples/Imp2Vir/CFGC_Interface.v
@@ -31,6 +31,17 @@ Section FreshnessMonad.
     unfold name. now apply neq_mk_anon.
   Qed.
 
+  Definition is_anon (b : block_id) : Prop :=
+    exists n, b = Anon n.
+
+  Lemma is_anon_name : forall n, is_anon (name n).
+  Proof.
+    intros.
+    unfold name, mk_anon.
+    unfold is_anon.
+    now eexists.
+  Qed.
+
   Record FST :=
     mk_FST
       {
@@ -169,12 +180,47 @@ Section CFG_LANG.
         mk_while expr_code cond dgB inB outB
     end.
 
+  Fixpoint len_entry_exit (cfg : cfg_lang) : (nat * nat) :=
+    match cfg with
+    | CBlock c => (1,1)
+    | CSeq c1 c2 =>
+        let '(i1,e1) := len_entry_exit c1 in
+        let '(i2,e2) := len_entry_exit c2 in
+        (i1+i2, e1+e2)
+    | CBranch _ c1 c2 =>
+        let '(i1,e1) := len_entry_exit c1 in
+        let '(i2,e2) := len_entry_exit c2 in
+        (i1+i2-1, e1+e2)
+    | CJoin c =>
+        let '(i,e) := len_entry_exit c in
+        (i, e-1)
+    | CWhile _ _ c => len_entry_exit c
+    end.
+
+  Definition wf_cfg_lang c :=
+    forall i e,
+    len_entry_exit c = (i,e) ->
+    i >= 1 /\ e >= 1.
+  From Vellvm Require Import Utils.Tactics.
+  From Coq Require Import Lia.
+
+  Lemma t :
+    forall c c1 i e,
+      c = CJoin c1 ->
+      wf_cfg_lang c ->
+      len_entry_exit c1 = (i,e) ->
+      e >= 2.
+  Admitted.
+
+
+  (* TODO I want to ensure that,
+     for CJoin c, len_entry_exit c = (i,e) -> e >= 2 (else it is not WF)
+   *)
+
 End CFG_LANG.
 
 
-From Vellvm Require Import Utils.Tactics.
 
-From Coq Require Import Lia.
 Require Import Coqlib.
 Require Import Util.
 
@@ -186,7 +232,12 @@ Definition wf_inputs (g : dcfg) : Prop :=
 
 Definition wf_outputs (g : dcfg) : Prop :=
   List.incl (outs g) (outputs (graph g))
-  /\ list_disjoint (outs g) (inputs (graph g)) .
+  /\ list_disjoint (outs g) (inputs (graph g))
+  /\ list_norepet (outs g).
+
+Definition wf_name (g : dcfg) : Prop :=
+  Forall (fun b => is_anon b ) (inputs (graph g))
+  /\ Forall (fun b => is_anon b ) (outputs (graph g)).
 
 Definition wf_graph (g : dcfg) : Prop :=
   wf_ocfg_bid (graph g).
@@ -194,7 +245,8 @@ Definition wf_graph (g : dcfg) : Prop :=
 Definition wf_dcfg (g : dcfg) : Prop :=
   wf_inputs g
   /\ wf_outputs g
-  /\ wf_graph g .
+  /\ wf_graph g
+  /\ wf_name g.
 
 Lemma wf_dcfg_ocfg : forall dg, wf_dcfg dg -> wf_ocfg_bid (graph dg).
 Proof.
@@ -202,297 +254,21 @@ Proof.
   unfold wf_dcfg, wf_graph in H ; intuition.
 Qed.
 
-Lemma wf_mk_block : forall σ c, wf_dcfg (snd ((mk_block c) σ )).
+
+Lemma snd_intro : forall {A B : Type} (p : A * B) x y, p = (x, y) -> snd p = y.
 Proof.
-  intros.
-  unfold wf_dcfg, wf_inputs, wf_outputs, mk_block, wf_graph, wf_ocfg_bid.
-  destruct σ ; cbn.
-  unfold incl.
-  intuition
-  ; try reflexivity
-  ; try (cbn in * ; assumption)
-  ; try apply List_norepet_singleton.
-  apply list_disjoint_singletons.
-  rewrite neq_name. lia.
+  intros. now inv H.
 Qed.
 
-Lemma wf_mk_seq : forall σ g1 g2 out1 in2,
-    independent_flows_dcfg g1 g2 ->
-    (outs g1) ⊍ (outs g2) ->
-    List.In out1 (outs g1) ->
-    List.In in2 (ins g2) ->
-    wf_dcfg g1 -> (* recursive use of the interface *)
-    wf_dcfg g2 ->
-    wf_dcfg (snd ((mk_seq g1 g2 out1 in2) σ )).
-Proof.
-  intros *  FLOWS DISJOINTS_OUTPUTS OUT IN WF_G1 WF_G2.
-  unfold wf_dcfg, wf_inputs, wf_outputs, mk_seq, wf_graph, wf_ocfg_bid.
-  destruct σ ; cbn.
-  unfold wf_dcfg, wf_inputs, wf_outputs, wf_graph, wf_ocfg_bid in WF_G1, WF_G2.
-  destruct WF_G1 as [INPUTS_G1 [[OUTPUTS_G1 DISJOINTS_G1] WF_BID_G1]].
-  destruct WF_G2 as [INPUTS_G2 [[OUTPUTS_G2 DISJOINTS_G2] WF_BID_G2]].
-  unfold incl.
-  simpl in *.
-  intuition ;
-    repeat flatten_all.
-  - unfold cfg_seq.
-    simpl in *.
-    break_list_goal.
-    break_list_hyp.
-    match goal with
-    | h: List.In _ _ \/ List.In _ _ |- _ => destruct h
-    end.
-    + left. now apply INPUTS_G1.
-    + right ; right.
-      apply INPUTS_G2.
-      now in_list_rem.
-  - unfold cfg_seq.
-    simpl in *.
-    break_list_goal.
-    break_list_hyp.
-    match goal with
-    | h: List.In _ _ \/ List.In _ _ |- _ => destruct h
-    end.
-    + left. apply OUTPUTS_G1.
-      now in_list_rem.
-    + right ; apply in_or_app ; right.
-      now apply OUTPUTS_G2.
-  - unfold cfg_seq.
-    simpl in *.
-    break_list_goal.
-    apply list_disjoint_app_r.
-    split
-    ; [ apply list_disjoint_app_l
-      | apply list_disjoint_app_r
-        ; split
-        ; apply list_disjoint_app_l
-      ] ; try split ; try assumption.
-    + now apply remove_disjoint.
-    + simpl.
-      unfold independent_flows_dcfg in FLOWS
-      ; simpl in FLOWS
-      ; unfold independent_flows in FLOWS
-      ; unfold no_reentrance in FLOWS.
-      destruct FLOWS as [FLOWS  [_ _]].
-      eapply incl_disjoint ; try eassumption.
-    + apply remove_disjoint_remove ; simpl.
-      rewrite eq_bid_refl.
-      apply list_disjoint_nil_r.
-    + simpl.
-      unfold independent_flows_dcfg in FLOWS
-      ; simpl in FLOWS
-      ; unfold independent_flows in FLOWS
-      ; unfold no_reentrance in FLOWS.
-      apply list_disjoint_cons_r ; [apply list_disjoint_nil_r|].
-      eapply list_disjoint_notin ; eassumption.
-    + simpl.
-      unfold independent_flows_dcfg in FLOWS
-      ; simpl in FLOWS
-      ; unfold independent_flows in FLOWS
-      ; unfold no_reentrance in FLOWS.
-      apply remove_disjoint.
-      destruct FLOWS as [_ [FLOWS _]].
-      eapply incl_disjoint ; try eassumption.
-  - unfold cfg_seq.
-    simpl in *.
-    break_list_goal.
-    simpl.
-    apply Coqlib.list_norepet_append
-    ; try assumption
-    ; unfold independent_flows_dcfg in FLOWS
-    ; simpl in FLOWS
-    ; unfold independent_flows in FLOWS
-    ; unfold no_reentrance in FLOWS.
-    + break_list_goal.
-      apply Coqlib.list_norepet_append ; try assumption.
-      apply List_norepet_singleton.
-      destruct FLOWS as [_ [FLOWS _]].
-      apply Util.list_disjoint_singleton_left.
-      clear IN INPUTS_G1 WF_BID_G1 INPUTS_G2 OUTPUTS_G2 WF_BID_G2.
-      eapply Coqlib.list_disjoint_notin.
-      2:{ eassumption. }
-      eapply incl_disjoint ; eassumption.
-    + destruct FLOWS as [_ [_ FLOWS]] ; unfold no_duplicate_bid in FLOWS.
-      apply Coqlib.list_disjoint_cons_r ; try assumption.
-      apply Util.list_disjoint_singleton_left.
-      clear -DISJOINTS_G1 OUT.
-      apply Util.list_disjoint_singleton_left.
-      eapply Coqlib.list_disjoint_notin ; eassumption.
-Admitted.
-
-Lemma wf_mk_join : forall σ g out1 out2,
-    wf_dcfg g ->
-    wf_dcfg (snd ((mk_join g out1 out2) σ)).
-Proof.
-  intros * WF_G.
-  unfold wf_dcfg, wf_inputs, wf_outputs, mk_seq, wf_graph, wf_ocfg_bid.
-  destruct σ ; cbn.
-  unfold wf_dcfg, wf_inputs, wf_outputs, wf_graph, wf_ocfg_bid in WF_G.
-  destruct WF_G as [INPUTS_G [[OUTPUTS_G DISJOINTS_G] WF_BID_G]].
-  unfold incl in *.
-  repeat flatten_all.
-  simpl in *.
-  intuition.
-  - inv Heq.
-    apply INPUTS_G in H.
-    unfold cfg_join.
-    break_list_goal.
-    now left.
-  - rewrite H0.
-    unfold cfg_join.
-    break_list_goal.
-    simpl ; intuition.
-  - unfold cfg_join.
-    break_list_goal.
-    inv Heq.
-    left.
-    apply OUTPUTS_G.
-    repeat in_list_rem.
-    assumption.
-  - unfold cfg_join.
-    break_list_goal.
-    simpl in *.
-    apply Coqlib.list_disjoint_cons_l.
-    (* I need lemmas about remove, but it should be easy here *)
-    admit.
-    (* freshness of (name counter_bid0)*)
-    admit.
-  - unfold cfg_join.
-    break_list_goal.
-    simpl in *.
-    apply Coqlib.list_norepet_append ; try assumption.
-    (* NOTE out1 ≠ out2 *)
-    (* ... should I need new wf property on outputs ? (no_repeat) *)
-    (* ... or hypothesis let to the programmer ? *)
-    admit.
-    (* NOTE Coqlib.list_disjoint (inputs graph0) [out1; out2] *)
-    (* I need 2 things:
-       - new hypothesis (out1, out2 ∈ (fst (outs dg)))
-          --> the programmer will have to prove that, but easy if he uses the
-              interface correctly
-       - new wf property on dcfg, st ∀ bk ∈ (fst (outs dg)), bk ∉ (graph dg)
-     *)
-    admit.
-Admitted.
-
-Lemma wf_mk_branch : forall σ cond gT gF inT inF,
-    wf_dcfg gT ->
-    wf_dcfg gF ->
-    wf_dcfg (snd ((mk_branch cond gT gF inT inF) σ)).
-Proof.
-  intros *  WF_GT WF_GF.
-
-  unfold wf_dcfg, wf_inputs, wf_outputs, mk_seq, wf_graph, wf_ocfg_bid.
-  destruct σ ; cbn.
-  unfold wf_dcfg, wf_inputs, wf_outputs, wf_graph, wf_ocfg_bid in WF_GT, WF_GF.
-  destruct WF_GT as [INPUTS_GT [[OUTPUTS_GT DISJOINTS_GT] WF_BID_GT]].
-  destruct WF_GF as [INPUTS_GF [[OUTPUTS_GF DISJOINTS_GF] WF_BID_GF]].
-  unfold incl in *.
-  simpl in *.
-  intuition ;
-    repeat flatten_all ; simpl in * ; try auto.
-  - intuition. right.
-    inv Heq0.
-    break_list_goal.
-    break_list_hyp.
-    match goal with
-    | h: List.In _ _ \/ List.In _ _ |- _ => destruct h
-    end
-    ; [left ; apply INPUTS_GT | right ; apply INPUTS_GF]
-    ; now in_list_rem.
-  - inv Heq.
-    break_list_goal.
-    break_list_hyp.
-    right.
-    break_list_goal.
-    match goal with
-    | h: List.In _ _ \/ List.In _ _ |- _ => destruct h
-    end
-    ; [left ; apply OUTPUTS_GT | right ; apply OUTPUTS_GF]
-    ; assumption.
-  - apply Coqlib.list_disjoint_cons_r.
-    (* NOTE Coqlib.list_disjoint (l0 ++ l2) (inputs (graph0 ++ graph1)*)
-    admit.
-    (* freshness (name counter_bid0)*)
-    admit.
-  - break_list_goal.
-    apply Coqlib.list_norepet_append ; try assumption.
-    apply List_norepet_singleton.
-    apply Coqlib.list_norepet_append ; try assumption.
-    (* NOTE: Coqlib.list_disjoint (inputs GT) (inputs GF) *)
-    admit.
-    apply Util.list_disjoint_singleton_left.
-    (* freshness (name counter_bid0) *)
-    admit.
-Admitted.
-
-Lemma wf_mk_while : forall σ expr_code cond gB inB outB,
-    List.In outB (outs gB) ->
-    wf_dcfg gB ->
-    wf_dcfg (snd ((mk_while expr_code cond gB inB outB) σ)).
-Proof.
-  intros * OUTPUT WF_G.
-  unfold wf_dcfg, wf_inputs, wf_outputs, mk_seq, wf_graph, wf_ocfg_bid.
-  destruct σ ; cbn.
-  unfold wf_dcfg, wf_inputs, wf_outputs, wf_graph, wf_ocfg_bid in WF_G.
-  destruct WF_G as [INPUTS_G [[OUTPUTS_G DISJOINTS_G] WF_BID_G]].
-  unfold incl in *.
-  repeat flatten_all.
-  simpl in *.
-  intuition.
-  - inv Heq.
-    right.
-    do 2 break_list_goal ; simpl.
-    left.
-    apply INPUTS_G.
-    now in_list_rem.
-  - rewrite H0.
-    clear.
-    do 2 (break_list_goal ; simpl).
-    left ; cbn ; intuition.
-  - inv Heq.
-    break_list_goal ; simpl.
-    right.
-    break_list_goal ; simpl.
-    left.
-    apply OUTPUTS_G.
-    now in_list_rem.
-  - break_list_goal.
-    simpl in *.
-    apply list_disjoint_cons_l.
-    + apply list_disjoint_cons_r.
-      * apply remove_disjoint_remove ; cbn.
-        rewrite CFGC_Utils.remove_app.
-        apply list_disjoint_app_r.
-        split ;
-          [apply remove_disjoint_remove
-           ; apply remove_disjoint ; assumption
-          | simpl ; rewrite eq_bid_refl
-            ; apply list_disjoint_nil_r].
-      * (* freshness (name counter_bid0) *)
-        admit.
-    + (* freshness (name counter_bid0) *)
-      admit.
-  (* NOTE: for freshness, I need hypothesis about intervals of
-         block_id in graphs *)
-  - break_list_goal.
-    simpl in *.
-    break_list_goal.
-    apply list_norepet_append ; try assumption.
-    apply List_norepet_singleton.
-    apply list_norepet_append ; try assumption.
-    apply List_norepet_singleton.
-    apply list_disjoint_singleton_right.
-    eapply list_disjoint_notin ; eassumption.
-    apply list_disjoint_singleton_left.
-    (* NOTE: freshness (name counter_bid0) *)
-    admit.
-Admitted.
+Ltac intro_snd_evaluate :=
+  match goal with
+  | h: evaluate ?c ?σ = (_,?dg) |- _ =>
+      apply snd_intro in h
+  end.
 
 
 
 Require Import Datatypes.
-
 Theorem inv_len_inputs : forall (σ: FST) (c : cfg_lang) (dg : dcfg),
     snd ((evaluate c) σ) = dg ->
     (length (ins dg) >= 1)%nat.
@@ -594,6 +370,335 @@ Proof.
 Qed.
 
 
+
+Theorem inv_wf_inputs_outputs : forall (σ: FST) (c : cfg_lang) (dg : dcfg),
+    snd ((evaluate c) σ) = dg ->
+    wf_inputs dg /\ List.incl (outs dg) (outputs (graph dg)).
+Proof.
+  intros *. revert σ dg.
+  unfold wf_inputs.
+  induction c ; intros ; simpl in *.
+  - unfold mk_block in H.
+    unfold freshLabel in H.
+    simpl in H.
+    repeat flatten_all.
+    simpl in *.
+    rewrite <- H.
+    unfold cfg_block ; cbn.
+    split ; apply incl_refl.
+  - unfold mk_seq in *.
+    simpl in *.
+    repeat flatten_all.
+    simpl in *.
+    unfold cfg_seq in *.
+    inv H.
+    simpl in *.
+    do 2 intro_snd_evaluate.
+    apply IHc1 in Heq.
+    apply IHc2 in Heq0.
+    simpl in *.
+    destruct Heq, Heq0.
+    unfold incl in *.
+    split ; intros
+    ; break_list_goal ; break_list_hyp
+    ; simpl in *.
+    destruct H3.
+    apply H in H3 ; intuition.
+    in_list_rem; apply H1 in H3 ; intuition.
+    destruct H3.
+    in_list_rem; apply H0 in H3; intuition.
+    apply H2 in H3; intuition.
+  - unfold mk_branch in *.
+    simpl in *.
+    repeat flatten_all.
+    simpl in *.
+    unfold cfg_branch in *.
+    inv H.
+    simpl in *.
+    do 2 intro_snd_evaluate.
+    apply IHc1 in Heq.
+    apply IHc2 in Heq0.
+    simpl in *.
+    destruct Heq, Heq0.
+    unfold incl in *.
+    split ; intros
+    ; break_list_goal
+    ; simpl in *.
+    destruct H3. intuition.
+    break_list_hyp.
+    destruct H3.
+    in_list_rem; apply H in H3 ; intuition.
+    in_list_rem; apply H1 in H3 ; intuition.
+    break_list_hyp.
+    destruct H3.
+    apply H0 in H3; intuition.
+    apply H2 in H3; intuition.
+  - unfold mk_join in *.
+    simpl in *.
+    repeat flatten_all.
+    simpl in *.
+    unfold cfg_join in *.
+    inv H.
+    simpl in *.
+    intro_snd_evaluate.
+    apply IHc in Heq.
+    simpl in *.
+    destruct Heq.
+    unfold incl in *.
+    split ; intros
+    ; break_list_goal
+    ; simpl in *.
+    apply H in H1 ; intuition.
+    destruct H1.
+    intuition.
+    do 2 in_list_rem ; apply H0 in H1 ; intuition.
+  - unfold mk_while in *.
+    simpl in *.
+    repeat flatten_all.
+    simpl in *.
+    unfold cfg_while_loop in *.
+    inv H.
+    simpl in *.
+    intro_snd_evaluate.
+    apply IHc in Heq.
+    simpl in *.
+    destruct Heq.
+    unfold incl in *.
+    split ; intros
+    ; break_list_goal
+    ; simpl in *.
+    destruct H1.
+    intuition.
+    in_list_rem ; apply H in H1 ; intuition.
+    destruct H1.
+    intuition.
+    in_list_rem ; apply H0 in H1 ; intuition.
+Qed.
+
+
+Theorem inv_name_anon : forall (σ: FST) (c : cfg_lang) (dg : dcfg),
+    snd ((evaluate c) σ) = dg ->
+    wf_name dg.
+Proof.
+  intros *. revert σ dg.
+  unfold wf_name.
+  pose proof inv_wf_inputs_outputs as INV_IN_OUT ;
+    unfold wf_inputs in INV_IN_OUT.
+  induction c ; intros ; simpl in H.
+  - admit.
+  - unfold mk_seq in H
+    ; repeat flatten_all
+    ; simpl in *.
+    inv H ; simpl.
+    unfold cfg_seq ; simpl.
+    repeat flatten_all ; simpl in *.
+    repeat intro_snd_evaluate.
+    match goal with
+    | h:context[snd (evaluate ?c ?σ) = ?dg] |- _ =>
+        let B := fresh "H" in
+        assert (B : snd (evaluate c σ) =  dg) by now rewrite h
+        (* ; apply INV_IN_OUT in B *)
+    end.
+    apply INV_IN_OUT in H ; destruct H.
+    apply IHc2 in Heq0 ; simpl in Heq0.
+   match goal with
+    | h:context[snd (evaluate ?c ?σ) = ?dg] |- _ =>
+        let B := fresh "H" in
+        assert (B : snd (evaluate c σ) =  dg) by now rewrite h
+        (* ; apply INV_IN_OUT in B *)
+    end.
+    apply INV_IN_OUT in H1 ; destruct H1.
+    apply IHc1 in Heq ; simpl in Heq.
+    simpl in *.
+    split
+    ; break_list_goal
+    (* ; rewrite !Forall_app *)
+    ; intuition
+    ; cbn
+    ; break_list_goal
+    ; rewrite !List.Forall_app
+    ; intuition
+    ; [apply incl_Forall with (l1 := outs0) | apply incl_Forall with (l1 := ins1)]
+    ; unfold incl ; intros
+    ; try (
+          match goal with | h: In _ [_] |- _ => apply In_singleton in h end
+          ; subst ; apply hd_In
+        ).
+    admit. (* true by invariant on length outs *)
+    eapply incl_Forall ; try eassumption.
+    admit. (* true by invariant on length ins *)
+    eapply incl_Forall ; try eassumption.
+  - admit.
+  - admit.
+  - admit.
+Admitted.
+
+Fixpoint max_bid' (l : list block_id) b :=
+  match l with
+  | [] => b
+  | h :: t => if leb_bid b h then max_bid' t h else max_bid' t b
+  end.
+
+Fixpoint min_bid' (l : list block_id) b :=
+  match l with
+  | [] => b
+  | h :: t => if leb_bid b h then min_bid' t b else min_bid' t h
+  end.
+
+Definition max_bid (l : list block_id) :=
+  max_bid' l (hd (Anon 0) l).
+
+Definition min_bid (l : list block_id) :=
+  min_bid' l (hd (Anon 0) l).
+
+Lemma leb_bid_refl : forall a, leb_bid a a = true.
+Admitted.
+
+
+Lemma max_bid_spec : forall l,
+    (length l >= 1)%nat ->
+    Forall (fun b => le_bid b (max_bid l)) l.
+Proof.
+  induction l ; try (now simpl).
+  intros.
+  apply Forall_cons.
+  unfold le_bid.
+  unfold max_bid ; simpl.
+  rewrite leb_bid_refl.
+Admitted.
+
+Lemma min_bid_spec : forall l,
+    (length l >= 1)%nat ->
+        Forall (fun b => le_bid (min_bid l) b) l.
+Admitted.
+
+Definition max_label (dg : dcfg) (max : block_id) :=
+  max_bid (inputs (graph dg) ++ outputs (graph dg)) = max.
+
+Definition min_label (dg : dcfg) (min : block_id) :=
+  min_bid (inputs (graph dg) ++ outputs (graph dg)) = min.
+
+Definition interval_label (dg : dcfg) (min max : block_id) :=
+  max_label dg max /\ min_label dg min.
+
+Lemma inv_counter_bid :
+  forall σ σ' (cb cb' : nat) (cr cr' : int) (c : cfg_lang) (dg : dcfg) min max,
+    σ = {| counter_bid := cb; counter_reg := cr |} ->
+    σ' = {| counter_bid := cb'; counter_reg := cr' |} ->
+    interval_label dg min max ->
+    (evaluate c) σ = (σ', dg) ->
+    le_bid (name cb') max.
+Proof.
+  induction c ; intros ; subst ; simpl in *.
+  - unfold mk_block in *.
+    unfold freshLabel, interval_label in *.
+    simpl in * ; repeat flatten_all ; simpl in *.
+    inv H2.
+    unfold cfg_block in H1.
+    unfold max_label, min_label in H1.
+    cbn in *.
+    rewrite Z.leb_refl in *.
+    match goal with
+    | h:context[ ?x <=? ?y ] |- _ =>
+        let H := fresh "H" in
+        assert (H : x <=? y = true) by admit
+        ; rewrite H in * ; clear H
+    end.
+    destruct H1 ; subst.
+    unfold le_bid.
+    admit. (* obviously true *)
+Admitted.
+
+Lemma inv_min_label :
+  forall σ σ' (cb cb' : nat) (cr cr' : int) (c : cfg_lang) (dg : dcfg) min max,
+    σ = {| counter_bid := cb; counter_reg := cr |} ->
+    σ' = {| counter_bid := cb'; counter_reg := cr' |} ->
+    interval_label dg min max ->
+    (evaluate c) σ = (σ', dg) ->
+    min = name cb.
+Proof.
+  induction c ; intros ; subst ; simpl in *.
+  - unfold mk_block in *.
+    unfold freshLabel, interval_label in *.
+    simpl in * ; repeat flatten_all ; simpl in *.
+    inv H2.
+    unfold cfg_block in H1.
+    unfold max_label, min_label in H1.
+    cbn in *.
+    rewrite Z.leb_refl in *.
+    match goal with
+    | h:context[ ?x <=? ?y ] |- _ =>
+        let H := fresh "H" in
+        assert (H : x <=? y = true) by admit
+        ; rewrite H in * ; clear H
+    end.
+    intuition.
+  - unfold mk_seq in H2
+    ; repeat flatten_all ; simpl in *.
+    inv H2.
+    (* eapply IHc1; try reflexivity ; try eassumption. *)
+    unfold cfg_seq in *.
+Admitted.
+
+ Theorem inv_interval_name :
+  forall (σ1 σ2 σ3: FST) (c1 c2 : cfg_lang) (dg1 dg2 : dcfg) min1 max1 min2 max2,
+    (evaluate c1) σ1 = (σ2, dg1) ->
+    (evaluate c2) σ2 = (σ3, dg2) ->
+    interval_label dg1 min1 max1 ->
+    interval_label dg2 min2 max2 ->
+    le_bid max1 min2.
+Proof.
+  induction c1 ; intros.
+  - (* CBlock, CBlock *)
+    simpl in *.
+    unfold mk_block in *.
+    unfold freshLabel in *.
+    simpl in *. repeat flatten_all ; cbn in *.
+    inv H. inv H0. (* inv Heq3. *) inv Heq. inv Heq0. (* inv Heq4. *)
+    unfold interval_label, max_label, min_label in H1.
+    unfold cfg_block in *.
+    simpl in *.
+    unfold outputs in H1.
+    simpl in *.
+    unfold successors in H1.
+    simpl in *.
+    unfold max_bid, min_bid in *.
+    simpl in *.
+    rewrite Z.leb_refl in *.
+    match goal with
+    | h:context[ ?x <=? ?y ] |- _ =>
+        let H := fresh "H" in
+        assert (H : x <=? y = true) by admit
+        ; rewrite H in * ; clear H
+    end.
+    intuition ; subst.
+    eapply inv_counter_bid.
+Admitted.
+
+Lemma inv_interval_independant :
+  forall dg1 dg2 min1 max1 min2 max2,
+    interval_label dg1 min1 max1 ->
+    interval_label dg2 min2 max2 ->
+    le_bid max1 min2 ->
+    independent_flows_dcfg dg1 dg2 /\ (outs dg1) ⊍ (outs dg2).
+Proof.
+  intros.
+  unfold independent_flows_dcfg, independent_flows,
+    interval_label, max_label, min_label in *.
+  destruct dg1, dg2.
+  simpl in *.
+  unfold no_reentrance, no_duplicate_bid.
+  assert ((length (inputs graph0 ++ outputs graph0) >= 1)%nat) by admit. (* true using the invariant*)
+  assert ((length (inputs graph1 ++ outputs graph1) >= 1)%nat) by admit. (* true using the invariant*)
+  apply max_bid_spec in H3.
+  apply min_bid_spec in H2.
+  destruct H, H0.
+  rewrite H4, H0 in *.
+  rewrite Forall_app in H2,H3.
+  intuition.
+Admitted.
+
+
 Theorem inv_independent_flows :
   forall (σ1 σ2 σ3: FST) (c1 c2 : cfg_lang) (dg1 dg2 : dcfg),
     (evaluate c1) σ1 = (σ2, dg1) ->
@@ -601,8 +706,14 @@ Theorem inv_independent_flows :
     independent_flows_dcfg dg1 dg2.
 Proof.
   intros.
-  unfold independent_flows_dcfg, independent_flows.
-Admitted.
+  pose proof (inv_interval_independant dg1 dg2).
+  unfold independent_flows_dcfg, independent_flows in *.
+  pose proof (inv_interval_name σ1 σ2 σ3 c1 c2 dg1 dg2).
+  eapply H1 in H2
+  ; try intuition.
+  all : eexists.
+  all : eexists.
+Qed.
 
 Theorem inv_disjoint_outputs :
   forall (σ1 σ2 σ3: FST) (c1 c2 : cfg_lang) (dg1 dg2 : dcfg),
@@ -611,7 +722,370 @@ Theorem inv_disjoint_outputs :
     (outs dg1) ⊍ (outs dg2).
 Proof.
   intros.
+  pose proof (inv_interval_independant dg1 dg2).
+  unfold independent_flows_dcfg, independent_flows in *.
+  pose proof (inv_interval_name σ1 σ2 σ3 c1 c2 dg1 dg2).
+  eapply H1 in H2
+  ; try intuition.
+  all : eexists.
+  all : eexists.
+Qed.
+
+
+Lemma wf_mk_block : forall σ c, wf_dcfg (snd ((mk_block c) σ )).
+Proof.
+  intros.
+  unfold wf_dcfg, wf_inputs, wf_outputs, mk_block, wf_graph, wf_ocfg_bid.
+  destruct σ ; cbn.
+  unfold incl.
+  intuition
+  ; try reflexivity
+  ; try (cbn in * ; assumption)
+  ; try apply List_norepet_singleton.
+  apply list_disjoint_singletons.
+  rewrite neq_name. lia.
+  unfold wf_name.
+  simpl.
+  split
+  ; apply Forall_cons
+  ; try apply is_anon_name
+  ; try apply Forall_nil.
+Qed.
+
+Lemma wf_mk_seq : forall σ g1 g2 out1 in2,
+    independent_flows_dcfg g1 g2 ->
+    (outs g1) ⊍ (outs g2) ->
+    List.In out1 (outs g1) ->
+    List.In in2 (ins g2) ->
+    wf_dcfg g1 -> (* recursive use of the interface *)
+    wf_dcfg g2 ->
+    wf_dcfg (snd ((mk_seq g1 g2 out1 in2) σ )).
+Proof.
+  intros *  FLOWS DISJOINTS_OUTPUTS OUT IN WF_G1 WF_G2.
+  unfold wf_dcfg, wf_inputs, wf_outputs, mk_seq, wf_graph, wf_ocfg_bid, wf_name.
+  destruct σ ; cbn.
+  unfold wf_dcfg, wf_inputs, wf_outputs, wf_graph, wf_ocfg_bid,wf_name in WF_G1, WF_G2.
+  destruct WF_G1 as [INPUTS_G1 [[OUTPUTS_G1 [DISJOINTS_G1 OUTS_NOREP_G1]] [WF_BID_G1 [NAME_IN_G1 NAME_OUT_G1]]]].
+  destruct WF_G2 as [INPUTS_G2 [[OUTPUTS_G2 [DISJOINTS_G2 OUTS_NOREP_G2]] [WF_BID_G2 [NAME_IN_G2 NAME_OUT_G2]]]].
+  unfold incl.
+  cbn in *.
+  intuition ; repeat flatten_all.
+  - unfold cfg_seq.
+    simpl in *.
+    break_list_goal.
+    break_list_hyp.
+    match goal with
+    | h: List.In _ _ \/ List.In _ _ |- _ => destruct h
+    end.
+    + left. now apply INPUTS_G1.
+    + right ; right.
+      apply INPUTS_G2.
+      now in_list_rem.
+  - unfold cfg_seq.
+    simpl in *.
+    break_list_goal.
+    break_list_hyp.
+    match goal with
+    | h: List.In _ _ \/ List.In _ _ |- _ => destruct h
+    end.
+    + left. apply OUTPUTS_G1.
+      now in_list_rem.
+    + right ; apply in_or_app ; right.
+      now apply OUTPUTS_G2.
+  - unfold cfg_seq.
+    simpl in *.
+    break_list_goal.
+    apply list_disjoint_app_r.
+    split
+    ; [ apply list_disjoint_app_l
+      | apply list_disjoint_app_r
+        ; split
+        ; apply list_disjoint_app_l
+      ] ; try split ; try assumption.
+    + now apply remove_disjoint.
+    + simpl.
+      unfold independent_flows_dcfg in FLOWS
+      ; simpl in FLOWS
+      ; unfold independent_flows in FLOWS
+      ; unfold no_reentrance in FLOWS.
+      destruct FLOWS as [FLOWS  [_ _]].
+      eapply incl_disjoint ; try eassumption.
+    + apply remove_disjoint_remove ; simpl.
+      rewrite eq_bid_refl.
+      apply list_disjoint_nil_r.
+    + simpl.
+      unfold independent_flows_dcfg in FLOWS
+      ; simpl in FLOWS
+      ; unfold independent_flows in FLOWS
+      ; unfold no_reentrance in FLOWS.
+      apply list_disjoint_cons_r ; [apply list_disjoint_nil_r|].
+      eapply list_disjoint_notin ; eassumption.
+    + simpl.
+      unfold independent_flows_dcfg in FLOWS
+      ; simpl in FLOWS
+      ; unfold independent_flows in FLOWS
+      ; unfold no_reentrance in FLOWS.
+      apply remove_disjoint.
+      destruct FLOWS as [_ [FLOWS _]].
+      eapply incl_disjoint ; try eassumption.
+  - unfold cfg_seq.
+    simpl in *.
+    apply list_norepet_append.
+    (* lemma with remove, but easy *)
+    admit.
+    assumption.
+    now eapply remove_disjoint.
+  - unfold cfg_seq ; simpl in *.
+    break_list_goal.
+    simpl.
+    apply Coqlib.list_norepet_append
+    ; try assumption
+    ; unfold independent_flows_dcfg in FLOWS
+    ; simpl in FLOWS
+    ; unfold independent_flows in FLOWS
+    ; unfold no_reentrance in FLOWS.
+    + break_list_goal.
+      apply Coqlib.list_norepet_append ; try assumption.
+      apply List_norepet_singleton.
+      destruct FLOWS as [_ [FLOWS _]].
+      apply Util.list_disjoint_singleton_left.
+      clear IN INPUTS_G1 WF_BID_G1 INPUTS_G2 OUTPUTS_G2 WF_BID_G2.
+      eapply Coqlib.list_disjoint_notin.
+      2:{ eassumption. }
+      eapply incl_disjoint ; eassumption.
+    + destruct FLOWS as [_ [_ FLOWS]] ; unfold no_duplicate_bid in FLOWS.
+      apply Coqlib.list_disjoint_cons_r ; try assumption.
+      apply Util.list_disjoint_singleton_left.
+      clear -DISJOINTS_G1 OUT.
+      apply Util.list_disjoint_singleton_left.
+      eapply Coqlib.list_disjoint_notin ; eassumption.
+  - simpl in *.
+    unfold cfg_seq ; simpl.
+    repeat intro_snd_evaluate.
+    (* apply IHc1 in Heq ; simpl in Heq. *)
+    (* apply IHc2 in Heq0 ; simpl in Heq0. *)
+    break_list_goal
+    ; rewrite !Forall_app
+    ; intuition
+    ; cbn.
+    eapply incl_Forall.
+    (* In out1 (outs _) => incl [out1] (outs _)*)
+    (* NOTE easy but tedious *)
+    admit.
+    admit.
+  - simpl in *.
+    unfold cfg_seq ; simpl.
+    repeat intro_snd_evaluate.
+    break_list_goal
+    ; rewrite !Forall_app
+    ; intuition
+    ; cbn.
+    eapply incl_Forall.
+    (* NOTE easy but tedious *)
+    admit.
+    admit.
 Admitted.
+
+Lemma wf_mk_join : forall σ g out1 out2,
+    out1 <> out2 ->
+    List.In out1 (outs g) ->
+    List.In out2 (outs g) ->
+    wf_dcfg g ->
+    wf_dcfg (snd ((mk_join g out1 out2) σ)).
+Proof.
+  intros * NEQ_OUTS OUT1_OUTS OUT2_OUTS WF_G.
+  unfold wf_dcfg, wf_inputs, wf_outputs, mk_seq, wf_graph, wf_ocfg_bid, wf_name.
+  destruct σ ; cbn.
+  unfold wf_dcfg, wf_inputs, wf_outputs, wf_graph, wf_ocfg_bid, wf_name in WF_G.
+  destruct WF_G as [INPUTS_G [[OUTPUTS_G [DISJOINTS_G OUTS_NOREP_G]] [WF_BID_G [NAME_IN_G NAME_OUT_G]]]].
+  unfold incl in *.
+  repeat flatten_all.
+  simpl in *.
+  intuition.
+  - inv Heq.
+    apply INPUTS_G in H.
+    unfold cfg_join.
+    break_list_goal.
+    now left.
+  - rewrite H0.
+    unfold cfg_join.
+    break_list_goal.
+    simpl ; intuition.
+  - unfold cfg_join.
+    break_list_goal.
+    inv Heq.
+    left.
+    apply OUTPUTS_G.
+    now repeat in_list_rem.
+  - unfold cfg_join.
+    break_list_goal.
+    simpl in *.
+    apply Coqlib.list_disjoint_cons_l.
+    apply remove_disjoint_remove.
+    (* easy but tedious *)
+    admit.
+    (* freshness of (name counter_bid0)*)
+    admit.
+  - unfold cfg_join.
+    break_list_goal.
+    simpl in *.
+    admit. (* NOTE easy but tedious + freshness counter_bid0 *)
+  - unfold cfg_join.
+    break_list_goal.
+    simpl in *.
+    apply Coqlib.list_norepet_append ; try assumption.
+    apply list_norepet_cons ; try apply List_norepet_singleton.
+    now rewrite In_singleton.
+    apply list_disjoint_sym.
+    apply incl_disjoint with (l1 := outs0) ; try assumption.
+    apply incl_cons ; try assumption.
+    apply incl_cons ; try assumption ; try apply incl_nil_l.
+  - admit. (* NOTE easy but tedious *)
+  - admit. (* NOTE easy but tedious *)
+Admitted.
+
+Lemma wf_mk_branch : forall σ cond gT gF inT inF,
+    independent_flows_dcfg gT gF ->
+    (outs gT) ⊍ (outs gF) ->
+    wf_dcfg gT ->
+    wf_dcfg gF ->
+    wf_dcfg (snd ((mk_branch cond gT gF inT inF) σ)).
+Proof.
+  intros *  INDEPENDENT_FLOWS DISJOINT_OUTS WF_GT WF_GF.
+  unfold wf_dcfg, wf_inputs, wf_outputs, mk_seq, wf_graph, wf_ocfg_bid, wf_name.
+  destruct σ ; cbn.
+  unfold wf_dcfg, wf_inputs, wf_outputs, wf_graph, wf_ocfg_bid, wf_name in WF_GT, WF_GF.
+  destruct WF_GT as [INPUTS_GT [[OUTPUTS_GT [DISJOINTS_GT NO_REP_GT]] [WF_BID_GT [NAME_IN_GT NAME_OUT_GT]]]].
+  destruct WF_GF as [INPUTS_GF [[OUTPUTS_GF [DISJOINTS_GF NO_REP_GF]] [WF_BID_GF [NAME_IN_GF NAME_OUT_GF]]]].
+  unfold incl in *.
+  simpl in *.
+  intuition ;
+    repeat flatten_all ; simpl in * ; try auto.
+  - intuition. right.
+    inv Heq0.
+    break_list_goal.
+    break_list_hyp.
+    match goal with
+    | h: List.In _ _ \/ List.In _ _ |- _ => destruct h
+    end
+    ; [left ; apply INPUTS_GT | right ; apply INPUTS_GF]
+    ; now in_list_rem.
+  - inv Heq.
+    break_list_goal.
+    break_list_hyp.
+    right.
+    break_list_goal.
+    match goal with
+    | h: List.In _ _ \/ List.In _ _ |- _ => destruct h
+    end
+    ; [left ; apply OUTPUTS_GT | right ; apply OUTPUTS_GF]
+    ; assumption.
+  - apply Coqlib.list_disjoint_cons_r.
+    unfold independent_flows_dcfg,independent_flows,no_reentrance in *
+    ; simpl in *.
+    break_list_goal.
+    apply list_disjoint_app_l.
+    split ; eapply list_disjoint_sym ; apply list_disjoint_app_l.
+    intuition.
+    eapply incl_disjoint ; [unfold incl ; intros ; eassumption
+                           | try assumption ; try  now apply list_disjoint_sym].
+    apply list_disjoint_sym.
+    eapply incl_disjoint with (l1 := outputs graph0) ; assumption.
+    intuition.
+    apply list_disjoint_sym.
+    eapply incl_disjoint with (l1 := outputs graph1) ; assumption.
+    eapply incl_disjoint ; [unfold incl ; intros ; eassumption
+                           | try assumption ; try  now apply list_disjoint_sym].
+    (* freshness (name counter_bid0)*)
+    admit.
+  - apply list_norepet_append ; assumption.
+  - break_list_goal.
+    apply Coqlib.list_norepet_append ; try assumption
+    ; try apply List_norepet_singleton.
+    + apply Coqlib.list_norepet_append ; try assumption.
+      unfold independent_flows_dcfg,independent_flows,no_duplicate_bid in *
+      ; simpl in *.
+      intuition.
+    + apply Util.list_disjoint_singleton_left.
+    (* freshness (name counter_bid0) *)
+    admit.
+  - admit.
+  - admit.
+Admitted.
+
+Lemma wf_mk_while : forall σ expr_code cond gB inB outB,
+    List.In outB (outs gB) ->
+    wf_dcfg gB ->
+    wf_dcfg (snd ((mk_while expr_code cond gB inB outB) σ)).
+Proof.
+  intros * OUTPUT WF_G.
+  unfold wf_dcfg, wf_inputs, wf_outputs, mk_seq, wf_graph, wf_ocfg_bid, wf_name.
+  destruct σ ; cbn.
+  unfold wf_dcfg, wf_inputs, wf_outputs, wf_graph, wf_ocfg_bid, wf_name in WF_G.
+  destruct WF_G as [INPUTS_G [[OUTPUTS_G [DISJOINTS_G NO_REP_G]] [WF_BID_G [NAME_IN_G NAME_OUT_G]]]].
+  unfold incl in *.
+  repeat flatten_all.
+  simpl in *.
+  intuition.
+  - inv Heq.
+    right.
+    do 2 break_list_goal ; simpl.
+    left.
+    apply INPUTS_G.
+    now in_list_rem.
+  - rewrite H0.
+    clear.
+    do 2 (break_list_goal ; simpl).
+    left ; cbn ; intuition.
+  - inv Heq.
+    break_list_goal ; simpl.
+    right.
+    break_list_goal ; simpl.
+    left.
+    apply OUTPUTS_G.
+    now in_list_rem.
+  - break_list_goal.
+    simpl in *.
+    apply list_disjoint_cons_l.
+    + apply list_disjoint_cons_r.
+      * apply remove_disjoint_remove ; cbn.
+        rewrite CFGC_Utils.remove_app.
+        apply list_disjoint_app_r.
+        split ;
+          [apply remove_disjoint_remove
+           ; apply remove_disjoint ; assumption
+          | simpl ; rewrite eq_bid_refl
+            ; apply list_disjoint_nil_r].
+      * (* freshness (name counter_bid0) *)
+        admit.
+    + (* freshness (name counter_bid0) *)
+      admit.
+  (* NOTE: for freshness, I need hypothesis about intervals of
+         block_id in graphs *)
+  - break_list_goal.
+    simpl in *.
+    break_list_goal.
+    apply list_norepet_append ; try assumption.
+    apply List_norepet_singleton.
+    admit. (* easy but tedious *)
+    apply list_disjoint_singleton_left.
+    admit. (* freshness counter_bid0 *)
+  - break_list_goal.
+    simpl in *.
+    break_list_goal.
+    apply list_norepet_append ; try assumption.
+    apply List_norepet_singleton.
+    apply list_norepet_append ; try assumption.
+    apply List_norepet_singleton.
+    apply list_disjoint_singleton_right.
+    eapply list_disjoint_notin ; eassumption.
+    apply list_disjoint_singleton_left.
+    (* NOTE: freshness (name counter_bid0) *)
+    admit.
+  - admit.
+  - admit.
+Admitted.
+
 
 Theorem wf_evaluate : forall (σ: FST) (c : cfg_lang) (dg : dcfg),
     snd ((evaluate c) σ) = dg ->
@@ -637,52 +1111,27 @@ Proof.
   - repeat flatten_all.
     rewrite <- H.
     apply wf_mk_branch.
+    + eapply inv_independent_flows ; eassumption.
+    + eapply inv_disjoint_outputs ; eassumption.
     + eapply IHc1. now erewrite Heq.
     + eapply IHc2. now erewrite Heq0.
   - repeat flatten_all.
     rewrite <- H.
     apply wf_mk_join.
-    eapply IHc. now erewrite Heq.
+    + admit. (* we have no_rep_outs thanks to WF + (hd l) and (hd (tl l))*)
+    + apply hd_In.
+      apply (inv_len_outputs σ c d). now rewrite Heq.
+    + admit. (* TODO we need WF on cfg_lang st JOIN can only take cfg_lang with at least 2 outputs *)
+    + eapply IHc. now erewrite Heq.
   - repeat flatten_all.
     rewrite <- H.
     apply wf_mk_while.
     + apply hd_In.
       apply (inv_len_outputs σ c d). now rewrite Heq.
     + eapply IHc. now erewrite Heq.
-Qed.
+Admitted.
 
 
-Lemma wf_mk_block_bind :
-  forall σ0 σ1 σ2 c1 c2 g1 g2,
-    (mk_block c1) σ0 = (σ1, g1) ->
-    (mk_block c2) σ1 = (σ2, g2) ->
-    independent_flows (graph g1) (graph g2).
-Proof.
-  intros.
-  unfold mk_block in *.
-  unfold freshLabel in *.
-  destruct σ0.
-  cbn in *.
-  inv H. inv H0.
-  simpl.
-  unfold independent_flows, no_duplicate_bid, no_reentrance.
-  unfold cfg_block.
-  cbn.
-  unfold Coqlib.list_disjoint.
-  intuition ; subst ;
-    repeat (
-        match goal with
-        | h:context[List.In _ [_]] |- _ => apply In_singleton in h
-        end
-      )
-  ; rewrite H0 in H ; clear H0
-  ; match goal with
-    | h:context[ name ?x = name ?y ] |- _ =>
-        assert (contra : name x <> name y)
-        by (apply neq_name ; lia )
-    end ;
-    now apply contra in H.
-Qed.
 
 Definition denote_dcfg (dg : dcfg) := denote_cfg (graph dg).
 Definition denote_cfg_lang (g : cfg_lang) (σ : FST) := denote_dcfg (snd ((evaluate g) σ)).
